ErasedQuant.v
@@ -4,6 +4,23 @@ Require Export SystemFR.ReducibilityOpenEquivalent.
 Opaque reducible_values.
 Opaque makeFresh.
 
+Lemma reducible_exists:
+  forall ρ t t' T1 T2,
+    valid_interpretation ρ ->
+    is_erased_type T2 ->
+    wf T2 1 ->
+    pfv T2 term_var = nil ->
+    [ ρ | t' : T1 ] ->
+    [ ρ | t : open 0 T2 t' ] ->
+    [ ρ | t : T_exists T1 T2 ].
+Proof.
+  unfold reducible, reduces_to;
+    repeat step.
+  exists v; repeat step || simp_red; eauto using reducible_values_closed.
+  exists v0; repeat step; t_closer.
+  eapply reducibility_values_ltr; eauto; steps; t_closer.
+Qed.
+
 Lemma reducible_forall:
   forall ρ t U V A,
     valid_interpretation ρ ->
