SubtypeNorm.v
@@ -19,23 +19,6 @@ Proof.
   eauto using open_subnormwiden_helper.
 Qed.
 
-Lemma open_subnorm_helper:
-  forall Θ Γ T1 T1' T1'' T2 T2' T2'',
-    [ Θ; Γ ⊨ T1 = T1' ] ->
-    [ Θ; Γ ⊨ T2 = T2' ] ->
-    untangle T1' T1'' ->
-    untangle T2' T2'' ->
-    [ Θ; Γ ⊨ T1'' <: T2'' ] ->
-    [ Θ; Γ ⊨ T1 <: T2 ].
-Proof.
-  intros.
-  eapply open_subtype_trans; eauto using open_equivalent_subtype.
-  eapply open_subtype_trans; eauto using open_equivalent_subtype, untangle_open_equivalent_types.
-  eapply open_subtype_trans; eauto.
-  eapply open_subtype_trans; eauto using open_equivalent_subtype_back.
-  eauto using open_equivalent_subtype_back, untangle_open_equivalent_types.
-Qed.
-
 Lemma open_subnorm:
   forall Γ T1 T1' T1'' T2 T2' T2'',
     [ Γ ⊨ T1 = T1' ] ->
@@ -45,5 +28,10 @@ Lemma open_subnorm:
     [ Γ ⊨ T1'' <: T2'' ] ->
     [ Γ ⊨ T1 <: T2 ].
 Proof.
-  eauto using open_subnorm_helper.
+  intros.
+  eapply open_subtype_trans; eauto using open_equivalent_subtype.
+  eapply open_subtype_trans; eauto using open_equivalent_subtype, untangle_open_equivalent_types.
+  eapply open_subtype_trans; eauto.
+  eapply open_subtype_trans; eauto using open_equivalent_subtype_back.
+  eauto using open_equivalent_subtype_back, untangle_open_equivalent_types.
 Qed.
